Splinter/Betree/Branches.i.dfy
@@ -30,6 +30,7 @@ module BranchesMod {
 		}
 
     predicate BranchesDisjoint()
+      requires (forall root | root in roots :: GetBranch(root).Acyclic())
     {
       && (forall r1, r2 | r1 in roots && r2 in roots && r1 != r2 :: 
         GetBranch(r1).ReachableAddrs() !! GetBranch(r2).ReachableAddrs())
@@ -74,137 +75,6 @@ module BranchesMod {
     {
       var branchDisk := DiskView(MapRestrict(diskView.entries, GetBranch(root).ReachableAddrs()));
       Branches(roots - {root}, diskView.RemoveDisk(branchDisk))
-    }
-
-    // TODO: why we needed this again lol we will see if we can use it for 
-    // ah it's easier to put things togther this way I think
-    // like a compose rankings thing
-    function GetTightBranch(addr: Address) : (branch: LinkedBranch)
-      requires WF()
-      requires ValidBranch(addr)
-      ensures branch.WF()
-      ensures branch.Acyclic()
-    {
-      var branch := GetBranch(addr);
-      var tightDisk := DiskView(MapRestrict(diskView.entries, branch.ReachableAddrs()));
-      var tightBranch := LinkedBranch(addr, tightDisk);
-
-      assert tightDisk.WF() by {
-        forall addr | addr in tightDisk.entries 
-          ensures tightDisk.NodeHasValidChildAddress(tightDisk.entries[addr])
-        {
-          branch.ReachableAddrClosed(branch.TheRanking(), addr);
-        }
-      }
-
-      assert tightBranch.Acyclic() by {
-        assert tightBranch.ValidRanking(branch.TheRanking());
-      }
-
-      tightBranch
-    }
-
-    lemma AddBranchWF(branch: LinkedBranch) 
-      requires AddBranch.requires(branch)
-      ensures AddBranch(branch).WF()
-    {
-      // see if this can help us
-      // GetTightBranch
-
-      // assert (exists ranking | (forall r | r in roots :: MapsAgree(ranking, GetBranch(r).))
-      
-      
-      
-      // )
-      // var  := AddBranch(branch);
-
-      
-
-      // let's merge it 
-      // var ranking :| (forall r | r in roots :: MapsAgree(ranking, GetBranch(r).TheRanking()));
-      
-      // GetBranch(r).ValidRanking(ranking));
-      //diskView.ValidRanking(ranking) && (forall r | r in roots :: r in ranking); 
-
-
-      assume false;
-
-      // forall addr | addr in ranking 
-      //   && addr in entries 
-
-
-
-
-      //  assert forall addr | addr in diskView.entries :: 
-      //       && addr in newBranches.diskView.entries 
-      //       && diskView.entries[addr] == newBranches.diskView.entries[addr];
-      // assert newBranches.diskView.WF();
-      // var newRanking := 
-
-      // forall root | root in newBranches.roots
-      //   ensures newBranches.GetBranch(root).Acyclic()
-      // {
-        // maybe before this step what we want to prove is that 
-        // ValidRanking
-
-
-        // is it easier if I show that each is disjoint?
-        // maybe I am dying percisely bc I don't have a disjoint clause
-        
-      //   if root == branch.root {
-      //     assume false;
-      //   } else {
-      //     var b := GetBranch(root);
-      //     var b' := newBranches.GetBranch(root);
-
-      //     var ranking := b.TheRanking();
-      //     assert b.ValidRanking(ranking);
-      //     assert b.diskView == diskView;
-
-      //     // valid ranking 
-      //     // assert forall r | r in ranking :: r in diskView.entries 
-    
-      //     forall addr | addr in ranking && addr in newBranches.diskView.entries 
-      //       ensures newBranches.diskView.NodeChildrenRespectsRank(ranking, addr)
-      //     {
-      //       assert addr in diskView.entries;
-      //       // if addr in diskView.entries 
-          
-      //       // assert diskView.NodeChildrenRespectsRank(ranking, addr);
-      //       assume false;
-      //     }
-
-
-        
-
-      //     assert b'.ValidRanking(ranking);
-      //     assert b'.Acyclic();
-          
-
-
-      //     assume false;
-
-      //     assert newBranches.GetBranch(root).ValidRanking(GetBranch(root).TheRanking());
-      //     assert newBranches.GetBranch(root).Acyclic();
-      //     // GetBranch()
-      //   }
-
-      //   // assume false;
-      // }
-
-      // forall root | root in newBranches.roots
-      //   ensures newBranches.GetBranch(root).AllKeysInRange()
-      // {
-      //   assume false;
-      // }
-    }
-     
-     lemma RemoveBranchWF(root: Address) 
-      requires RemoveBranch.requires(root)
-      ensures RemoveBranch(root).WF() 
-    {
-      assume false;
-
     }
 	}
 }
